valid_synth_parse_synth_recip

tests/layeff/LowParseWriters.Parsers.fst
@@ -88,6 +88,18 @@ let valid_synth_parse_synth
   );
 }
 
+let valid_synth_parse_synth_recip
+  p1 #t2 f2 f1 sq
+= {
+  valid_synth_valid = (fun h b pos pos' ->
+    LP.synth_injective_synth_inverse_synth_inverse_recip f2 f1 ();
+    LP.valid_synth h (get_parser p1) f2 (LP.make_slice b (B.len b)) pos
+  );
+  valid_synth_size = (fun x ->
+    LP.serialize_synth_eq (get_parser p1) f2 (dsnd p1).serializer f1 () (x)
+  );
+}
+
 let parse_vldata
   p min max
 =
